xor est correctement implementé ! (bon, il reste les admits...)

src/int63/CnfInt63.v
@@ -105,7 +105,7 @@ Section Checker.
      * ite_pos1         : {(not (if_then_else a b c)) a c}
      * ite_neg1         : {(if_then_else a b c) a (not c)} *)
 
-  Definition check_BuildDefInt lits i :=
+  Definition check_BuildDefInt lits :=
     let n := PArray.length lits in
     match get_form (Lit.blit (lits.[0])) with
     | Fatom a => 
@@ -147,7 +147,7 @@ Section Checker.
               | (Fatom a1,Fatom a2) =>
                 match (get_atom a1,get_atom a2) with
                 | (Auop (UO_index i2) h1', Auop (UO_index i3) h2') => 
-                  if (h1' == h1)&&(h2 == h2')&&(i1 ==i2)&&(i2 == i3)&&(i == i1)&&(Lit.is_pos (lits.[1]))&&(Lit.is_pos (lits.[2]))
+                  if (h1' == h1)&&(h2 == h2')&&(i1 ==i2)&&(i2 == i3)&&(Lit.is_pos (lits.[1]))&&(Lit.is_pos (lits.[2]))
                   then (
                     if (Lit.is_pos (lits.[0]))
                     then lits.[0]::lits.[1]::(Lit.neg (lits.[2]))::nil
@@ -168,7 +168,50 @@ Section Checker.
       end
    | _ => C._true
    end.
-
+   
+   (* * xor_pos2          : {(not (xor a b)) (not a) (not b)}
+     * xor_neg2          : {(xor a b) (not a) b}
+     * equiv_pos2        : {(not (iff a b)) (not a) b}
+     * equiv_neg2        : {(iff a b) a b}
+     * ite_pos2          : {(not (if_then_else a b c)) (not a) b}
+     * ite_neg2          : {(if_then_else a b c) (not a) (not b)} *)
+    Definition check_BuildDefInt2 lits :=
+    let n := PArray.length lits in
+    match get_form (Lit.blit (lits.[0])) with
+    | Fatom a => 
+      match get_atom a with
+      | Auop (UO_index i1) hxor =>
+        match get_atom hxor with
+        | Abop b h1 h2 =>
+          match (b) with
+          | (BO_int_xor) =>
+            if n == 3
+            then (
+              match (get_form (Lit.blit (lits.[1])),get_form (Lit.blit (lits.[2]))) with
+              | (Fatom a1,Fatom a2) =>
+                match (get_atom a1,get_atom a2) with
+                | (Auop (UO_index i2) h1', Auop (UO_index i3) h2') => 
+                  if (h1' == h1)&&(h2 == h2')&&(i1 ==i2)&&(i2 == i3)&&(Lit.is_pos (lits.[1]))&&(Lit.is_pos (lits.[2]))
+                  then (
+                    if (Lit.is_pos (lits.[0]))
+                    then lits.[0]::(Lit.neg (lits.[1]))::lits.[2]::nil
+                    else lits.[0]::(Lit.neg (lits.[1]))::(Lit.neg (lits.[2]))::nil
+                       )
+                  else C._true   
+                | _ => C._true
+                end
+              | _ => C._true
+              end
+                 )
+            else C._true
+          | _ => C._true
+          end
+        | _ => C._true
+        end
+      | _ => C._true
+      end
+   | _ => C._true
+   end.
 
   Definition check_BuildProjInt lits i :=
     let n := PArray.length lits in
@@ -176,19 +219,15 @@ Section Checker.
     | Fatom a => 
       match get_atom a with
       | Abop b h1 h2 => 
-        match (b,get_atom h1,get_atom h2) with
-        | (BO_eq t,Acop (CO_int x),Acop (CO_int y)) => 
+        match (b) with
+        | (BO_eq Typ.Tint) => 
           let test_correct i0 l :=
             match get_form (Lit.blit l) with
             | Fiff l1 l2 =>
               match (get_form (Lit.blit l1),get_form (Lit.blit l2)) with
               | (Fatom a1,Fatom a2) =>
                 match (get_atom a1,get_atom a2) with
-                | (Auop (UO_index j) hx1,Auop (UO_index k) hy1) => 
-                  match (get_atom hx1,get_atom hy1) with
-                  | (Acop (CO_int x1),Acop (CO_int y1)) => (n == Int63Op.digits + 1)&&(i < Int63Op.digits)&&(Lit.is_pos l1)&&(Lit.is_pos l2)&&(negb (Lit.is_pos (lits.[0])))&&(Lit.is_pos l)&&(Typ.eqb t Typ.Tint)&&(j == i0)&&(k == j)&&(x == x1)&&(y==y1)
-                  | _ => false
-                  end
+                | (Auop (UO_index j) h1',Auop (UO_index k) h2') => (n == Int63Op.digits + 1)&&(i < Int63Op.digits)&&(Lit.is_pos l1)&&(Lit.is_pos l2)&&(negb (Lit.is_pos (lits.[0])))&&(Lit.is_pos l)&&(j == i0)&&(k == j)&&(h1 == h1')&&(h2'==h2)
                 | _ => false
                 end
               | _ => false
@@ -283,48 +322,38 @@ Section Checker.
     Proof.
       unfold check_BuildProjInt,C.valid. intros lits i.
       
-      case_eq (t_form.[Lit.blit (lits.[0])]);intros i0; auto using C.interp_true.
-      case_eq (t_atom.[i0]);intros b; auto using C.interp_true.
-      case_eq b; intros t H i1 i2 H0; auto using C.interp_true; intro H1.
-      case_eq (t_atom.[i1]);intros c H2; auto using C.interp_true.
-      case_eq c;intros i3; auto using C.interp_true; intro H3.
-      case_eq (t_atom.[i2]);intros c0 H4; auto using C.interp_true.
-      case_eq c0;intro i4; auto using C.interp_true;intro H5.
-      case_eq (t_form.[Lit.blit (lits.[i+1])]);intros i5;auto using C.interp_true;intros i6 H6.
-      case_eq (t_form.[Lit.blit i5]);intro i7;auto using C.interp_true;intro H7.
-      case_eq (t_form.[Lit.blit i6]);intro i8;auto using C.interp_true; intro H8.
-      case_eq (t_atom.[i7]);intros u i9;auto using C.interp_true; intros H9.
-      case_eq u;intro i10;auto using C.interp_true;intro H10.
-      case_eq (t_atom.[i8]);intros u0 i11;auto using C.interp_true;intro H11.
-      case_eq u0;intro i12;auto using C.interp_true;intro H12.
-      case_eq (t_atom.[i9]);intros c1 H13;auto using C.interp_true.
-      case_eq c1;intros i13;auto using C.interp_true; intro H14.
-      case_eq (t_atom.[i11]);intros c2 H15;auto using C.interp_true.
-      case_eq c2;intro i14;auto using C.interp_true;intro H16.
+      case_eq (t_form.[Lit.blit (lits.[0])]);[intros a H|intro H|intro H|intros z1 z2 H|intros z1 H|intros z1 H|intros z1 H|intros z1 z2 H|intros z1 z2 H|intros z1 z2 z3 H]; auto using C.interp_true.
+      case_eq (t_atom.[a]);[intros z1 H1|intros z1 z2 H1|intros b h1 h2 H1|intros z1 z2 H1|intros z1 z2 H1]; auto using C.interp_true.
+      case_eq b; intro t; auto using C.interp_true;intro H3.
+      case_eq t;intro H4;auto using C.interp_true;subst t.
+      case_eq (t_form.[Lit.blit (lits.[i+1])]);[intros z1 H4|intros H4|intros H4|intros z1 z2 H4|intros z1 H4|intros z1 H4|intros z1 H4|intros z1 z2 H4|intros l1 l2 H4|intros z1 z2 z3 H4];auto using C.interp_true.
+      case_eq (t_form.[Lit.blit l1]);[intros a1 H8|intros H8|intros H8|intros z1 z2 H8|intros z1 H8|intros z1 H8|intros z1 H8|intros z1 z2 H8|intros z1 z2 H8|intros z1 z2 z3 H8];auto using C.interp_true.
+      case_eq (t_form.[Lit.blit l2]);[intros a2 H9|intros H9|intros H9|intros z1 z2 H9|intros z1 H9|intros z1 H9|intros z1 H9|intros z1 z2 H9|intros z1 z2 H9|intros z1 z2 z3 H9];auto using C.interp_true.
+      case_eq (t_atom.[a1]);[intros z1 H5|intros u1 h1' H5|intros z1 z2 z3 H5|intros z1 z2 H5|intros z1 z2 H5];auto using C.interp_true.
+      case_eq u1; intro j; auto using C.interp_true;intro H6.
+      case_eq (t_atom.[a2]);[intros z1 H7|intros u2 h2' H7|intros z1 z2 z3 H7|intros z1 z2 H7|intros z1 z2 H7];auto using C.interp_true.
+      case_eq u2; intro k; auto using C.interp_true;intro H10.
 
-      case_eq ((length lits == digits + 1) && (i < digits) && Lit.is_pos i5 && Lit.is_pos i6 && negb (Lit.is_pos (lits .[ 0])) && Lit.is_pos (lits .[ i + 1]) && Typ.eqb t Typ.Tint && (i10 == i) && (i12 == i10) && (i3 == i13) && (i4 == i14));intro H17.
-      apply andb_true_iff in H17; destruct H17 as (H17,H18); apply andb_true_iff in H17; destruct H17 as (H17,H19); apply andb_true_iff in H17; destruct H17 as (H17,H20); apply andb_true_iff in H17; destruct H17 as (H17,H21); apply andb_true_iff in H17; destruct H17 as (H17,H22); apply andb_true_iff in H17; destruct H17 as (H17,H23); apply andb_true_iff in H17; destruct H17 as (H17,H24); apply andb_true_iff in H17; destruct H17 as (H17,H25); apply andb_true_iff in H17; destruct H17 as (H17,H26); apply andb_true_iff in H17; destruct H17 as (H17,H27).
+      case_eq ((length lits == digits + 1) && (i < digits) && Lit.is_pos l1 && Lit.is_pos l2 && negb (Lit.is_pos (lits .[ 0])) && Lit.is_pos (lits .[ i + 1]) && (j == i) && (k == j) && (h1 == h1') &&(h2' == h2));intro H17;auto using C.interp_true.
+      apply andb_true_iff in H17; destruct H17 as (H17,H18); apply andb_true_iff in H17; destruct H17 as (H17,H19); apply andb_true_iff in H17; destruct H17 as (H17,H20); apply andb_true_iff in H17; destruct H17 as (H17,H21); apply andb_true_iff in H17; destruct H17 as (H17,H22); apply andb_true_iff in H17; destruct H17 as (H17,H23); apply andb_true_iff in H17; destruct H17 as (H17,H24); apply andb_true_iff in H17; destruct H17 as (H17,H25); apply andb_true_iff in H17; destruct H17 as (H17,H26).
       
-      rewrite Int63Properties.eqb_spec in H19; rewrite Int63Properties.eqb_spec in H20; rewrite Int63Properties.eqb_spec in H21; rewrite Int63Properties.eqb_spec in H18;apply Typ.eqb_spec in H22;subst i10; subst i12; subst i13; subst i14;subst t.
-      rewrite <- H3 in H14; rewrite <- H5 in H16; rewrite <- H10 in H12;subst u0; subst c1; subst c2.
-      rewrite negb_true_iff in H24.
+      rewrite Int63Properties.eqb_spec in H19; rewrite Int63Properties.eqb_spec in H20; rewrite Int63Properties.eqb_spec in H21; rewrite Int63Properties.eqb_spec in H18;rewrite Int63Properties.eqb_spec in H17;subst h1'; subst h2'; subst j; subst k.
+      rewrite <- H6 in H10;subst u2.
+      rewrite negb_true_iff in H23.
       
       simpl; rewrite orb_false_r; apply orb_true_iff.
-      unfold Lit.interp; rewrite H24; rewrite H23; rewrite negb_true_iff; unfold Var.interp; rewrite !rho_interp; rewrite H6; rewrite H1.
-      simpl; unfold Lit.interp; rewrite H25; rewrite H26; unfold Var.interp; rewrite !rho_interp; rewrite H8; rewrite H7;simpl.
-      unfold Atom.interp_form_hatom; unfold interp_hatom; rewrite !t_interp_wf. 
-      rewrite H0; rewrite H9;rewrite H11; simpl; rewrite !t_interp_wf.
-      unfold interp_uop; unfold interp_bop; rewrite H10; simpl; rewrite H2;rewrite H4;rewrite H13;rewrite H15; simpl; unfold interp_cop; rewrite H3;rewrite H5;simpl.
-      apply bool_impl; intro H28; apply Int63Properties.eqb_spec in H28; subst i4; trivial; apply Bool.eqb_true_iff; trivial.
-      
-      apply wf_t_atom. apply def_t_atom. 
-      apply wf_t_atom. apply def_t_atom.
-      apply wf_t_atom. apply def_t_atom.
-      apply wf_t_atom. apply def_t_atom.
-      apply wf_t_atom. apply def_t_atom.
-      apply wf_t_atom. apply def_t_atom.
-      apply wf_t_atom. apply def_t_atom. 
-      auto using C.interp_true.
+      unfold Lit.interp; rewrite H22; rewrite H23; rewrite negb_true_iff; unfold Var.interp; rewrite !rho_interp; rewrite H4; rewrite H.
+      simpl; unfold Lit.interp; rewrite H25; rewrite H24; unfold Var.interp; rewrite !rho_interp; rewrite H8; rewrite H9;simpl.
+      unfold Atom.interp_form_hatom; unfold interp_hatom; rewrite !t_interp_wf;try (apply wf_t_atom);try (apply def_t_atom). 
+      rewrite H5; rewrite H7;rewrite H1; simpl; rewrite !t_interp_wf;try (apply wf_t_atom);try (apply def_t_atom).
+      unfold interp_uop; unfold interp_bop; rewrite H6;rewrite H3; simpl; unfold apply_binop;unfold apply_unop.
+      case_eq (interp_atom (t_atom.[h1])); intros t1 v1 H10.
+      case_eq (interp_atom (t_atom.[h2])); intros t2 v2 H11.
+      case_eq (Typ.cast t1 Typ.Tint); [intros k1 H12| intros H12]. 
+      case_eq (Typ.cast t2 Typ.Tint); [intros k2 H13| intros H13].
+      simpl;apply bool_impl; intro H28; apply Int63Properties.eqb_spec in H28;rewrite H28; apply Bool.eqb_true_iff; trivial.
+      admit.
+      admit.
     Qed.
 
     Lemma digit_plus_1_not_0 : (0 == digits+1) = false.
@@ -384,70 +413,59 @@ Section Checker.
       apply not_0_ltb;apply succ_max_int;apply H1.
     Qed.
 
-    Lemma valid_check_BuildDefInt : forall lits i, C.valid rho (check_BuildDefInt lits i).
+    Lemma valid_check_BuildDefInt : forall lits, C.valid rho (check_BuildDefInt lits).
     Proof.
-      unfold check_BuildDefInt,C.valid; intros lits i.
+      unfold check_BuildDefInt,C.valid; intros lits.
       
-      case_eq (t_form .[ Lit.blit (lits .[ 0])]); intros i0; auto using C.interp_true; intro H.
-      case_eq (t_atom.[i0]);intros c i1; auto using C.interp_true. intros H0.
-      case_eq c;intro i2;auto using C.interp_true;intro H1.
-      case_eq (t_atom .[ i1]);intros c0 i3; auto using C.interp_true;intros i4 H2.
-      case_eq (c0);intro H3;auto using C.interp_true.
-      case_eq (length lits == 3); intros H9; auto using C.interp_true. 
-      case_eq (t_form .[ Lit.blit (lits .[ 1])]); intros i7; auto using C.interp_true; intro H10.
-      case_eq (t_form .[ Lit.blit (lits .[ 2])]); intros i8; auto using C.interp_true; intro H11.
-      case_eq (t_atom .[ i7]);intros c4 i12; auto using C.interp_true;intro H15.
-      case_eq c4;intro i13;auto using C.interp_true; intro H16.
-      case_eq (t_atom .[ i8]);intros c5 i17; auto using C.interp_true; intro H17.
-      case_eq c5;intro i14;auto using C.interp_true; intro H18.
-      case_eq ((i12 == i3) && (i4 == i17) && (i2 == i13) && (i13 == i14) && (i == i2) &&Lit.is_pos (lits .[ 1]) && Lit.is_pos (lits .[ 2]));intros H23.
-      apply andb_true_iff in H23; destruct H23 as (H23,H31);apply andb_true_iff in H23; destruct H23 as (H23,H26);apply andb_true_iff in H23; destruct H23 as (H23,H27);apply andb_true_iff in H23; destruct H23 as (H23,H28);apply andb_true_iff in H23; destruct H23 as (H23,H29);apply andb_true_iff in H23; destruct H23 as (H23,H30).
-      apply Int63Properties.eqb_spec in H23;apply Int63Properties.eqb_spec in H27;apply Int63Properties.eqb_spec in H28;apply Int63Properties.eqb_spec in H29;apply Int63Properties.eqb_spec in H30;subst i2; subst i13;subst i14;subst i17;subst i12. rewrite <- H1 in H16;rewrite <- H1 in H18; subst c4; subst c5.
+      case_eq (t_form .[ Lit.blit (lits .[ 0])]); [intros a H|intro H|intro H|intros z1 z2 H|intros z1 H|intros z1 H|intros z1 H|intros z1 z2 H|intros z1 z2 H|intros z1 z2 z3 H]; auto using C.interp_true.
+      case_eq (t_atom.[a]);[intros z1 H0|intros c hxor H0|intros c h1 h2 H0|intros z1 z2 H0|intros z1 z2 H0]; auto using C.interp_true.
+      case_eq c;intro i1;auto using C.interp_true;intro H1.
+      case_eq (t_atom.[hxor]);[intros z1 H2|intros z1 z2 H2|intros b h1 h2 H2|intros z1 z2 H2|intros z1 z2 H2];auto using C.interp_true.
+      case_eq b; intro H3;auto using C.interp_true.
+      case_eq (length lits == 3); intros H4; auto using C.interp_true. 
+      case_eq (t_form .[ Lit.blit (lits .[ 1])]);[intros a1 H5|intros|intros|intros|intros|intros|intros|intros|intros|intros]; auto using C.interp_true.
+      case_eq (t_form .[ Lit.blit (lits .[ 2])]);[intros a2 H6|intros|intros|intros|intros|intros|intros|intros|intros|intros]; auto using C.interp_true.
+      case_eq (t_atom .[ a1]);[intros|intros c1 h1' H7|intros|intros|intros]; auto using C.interp_true.
+      case_eq c1;intro i2;auto using C.interp_true; intro H8.
+      case_eq (t_atom .[ a2]);[intros|intros c2 h2' H9|intros|intros|intros]; auto using C.interp_true.
+      case_eq c2;intro i3;auto using C.interp_true;intro H10.
+      case_eq ((h1' == h1) && (h2 == h2') && (i1 == i2) && (i2 == i3) && Lit.is_pos (lits .[ 1]) && Lit.is_pos (lits .[ 2])); auto using C.interp_true;intros H23.
+      apply andb_true_iff in H23; destruct H23 as (H23,H31);apply andb_true_iff in H23; destruct H23 as (H23,H26);apply andb_true_iff in H23; destruct H23 as (H23,H27);apply andb_true_iff in H23; destruct H23 as (H23,H29);apply andb_true_iff in H23; destruct H23 as (H23,H30).
+      apply Int63Properties.eqb_spec in H23;apply Int63Properties.eqb_spec in H27;apply Int63Properties.eqb_spec in H29;apply Int63Properties.eqb_spec in H30; subst h1';subst h2';subst i2;subst i3. rewrite <- H1 in H10;rewrite <- H1 in H8; subst c1; subst c2.
       
       case_eq (Lit.is_pos (lits.[0]));intro H14.
       
       simpl; rewrite orb_false_r; apply orb_true_iff; rewrite orb_true_iff.
-      unfold Lit.interp; rewrite H26; rewrite H14; rewrite Lit.is_pos_neg; rewrite H31; simpl; unfold Var.interp; rewrite !rho_interp; rewrite Lit.blit_neg; rewrite H;rewrite H11;rewrite H10; simpl; unfold Atom.interp_form_hatom; unfold interp_hatom; rewrite !t_interp_wf.
-      rewrite H0;rewrite H17;rewrite H15; simpl; unfold interp_uop; rewrite H1; rewrite !t_interp_wf.
-      rewrite H2; simpl; rewrite !t_interp_wf. 
-      unfold interp_bop; rewrite H3;simpl. unfold apply_binop.
-      Check (interp_atom (t_atom .[ i3])).
-      case_eq (interp_atom (t_atom.[i3])); intros t1' v1 H32.
-      case_eq (interp_atom (t_atom.[i4])); intros t2' v2 H33.
+      unfold Lit.interp; rewrite H26; rewrite H14; rewrite Lit.is_pos_neg; rewrite H31; simpl; unfold Var.interp; rewrite !rho_interp; rewrite Lit.blit_neg; rewrite H;rewrite H5;rewrite H6; simpl; unfold Atom.interp_form_hatom; unfold interp_hatom; rewrite !t_interp_wf;try (apply wf_t_atom);try (apply def_t_atom).
+      rewrite H0;rewrite H7;rewrite H9; simpl; unfold interp_uop; rewrite H1; rewrite !t_interp_wf;try (apply wf_t_atom);try (apply def_t_atom).
+      rewrite H2; simpl; rewrite !t_interp_wf;try (apply wf_t_atom);try (apply def_t_atom).
+      unfold interp_bop; rewrite H3;simpl; unfold apply_binop.
+      case_eq (interp_atom (t_atom.[h1])); intros t1' v1 H32.
+      case_eq (interp_atom (t_atom.[h2])); intros t2' v2 H33.
       case_eq (Typ.cast t1' Typ.Tint); intros k. intro H34.
       case_eq (Typ.cast t2' Typ.Tint); intros k0. intro H35.
-      simpl;rewrite H34;rewrite H35;simpl.
-
-      unfold bit_rev. rewrite lxor_spec;destruct (bit (k (Typ.interp t_i) v1) i);destruct (bit (k0 (Typ.interp t_i) v2) i);[right;left|left|left|right;right];trivial.
+      simpl;rewrite H34;rewrite H35;simpl;unfold bit_rev;rewrite lxor_spec;destruct (bit (k (Typ.interp t_i) v1) i1);destruct (bit (k0 (Typ.interp t_i) v2) i1);[right;left|left|left|right;right];trivial.
 
       admit.
       admit.
-
-      apply wf_t_atom. apply def_t_atom. apply wf_t_atom. apply def_t_atom. apply wf_t_atom. apply def_t_atom. apply wf_t_atom. apply def_t_atom. apply wf_t_atom. apply def_t_atom. apply wf_t_atom. apply def_t_atom. apply wf_t_atom. apply def_t_atom. apply wf_t_atom. apply def_t_atom.
       
       simpl; rewrite orb_false_r; apply orb_true_iff; rewrite orb_true_iff.
-      unfold Lit.interp; rewrite H26; rewrite H14; rewrite H31; simpl; unfold Var.interp; rewrite !rho_interp; rewrite H;rewrite H11;rewrite H10; simpl; unfold Atom.interp_form_hatom; unfold interp_hatom; rewrite !t_interp_wf.
-      rewrite H0;rewrite H17;rewrite H15; simpl; unfold interp_uop; rewrite H1; rewrite !t_interp_wf.
-      rewrite H2; simpl; rewrite !t_interp_wf. 
-      unfold interp_bop; rewrite H3;simpl. unfold apply_binop.
-      Check (interp_atom (t_atom .[ i3])).
-      case_eq (interp_atom (t_atom.[i3])); intros t1' v1 H32.
-      case_eq (interp_atom (t_atom.[i4])); intros t2' v2 H33.
+      unfold Lit.interp; rewrite H26; rewrite H14;rewrite H31; simpl; unfold Var.interp; rewrite !rho_interp;rewrite H;rewrite H5;rewrite H6; simpl; unfold Atom.interp_form_hatom; unfold interp_hatom; rewrite !t_interp_wf;try (apply wf_t_atom);try (apply def_t_atom).
+      rewrite H0;rewrite H7;rewrite H9; simpl; unfold interp_uop; rewrite H1; rewrite !t_interp_wf;try (apply wf_t_atom);try (apply def_t_atom).
+      rewrite H2; simpl; rewrite !t_interp_wf;try (apply wf_t_atom);try (apply def_t_atom).
+      unfold interp_bop; rewrite H3;simpl; unfold apply_binop.
+      case_eq (interp_atom (t_atom.[h1])); intros t1' v1 H32.
+      case_eq (interp_atom (t_atom.[h2])); intros t2' v2 H33.
       case_eq (Typ.cast t1' Typ.Tint); intros k. intro H34.
       case_eq (Typ.cast t2' Typ.Tint); intros k0. intro H35.
-      simpl;rewrite H34;rewrite H35;simpl.
-
-      unfold bit_rev. rewrite lxor_spec;destruct (bit (k (Typ.interp t_i) v1) i);destruct (bit (k0 (Typ.interp t_i) v2) i);[left|right;left|right;right|left];trivial.
+      simpl;rewrite H34;rewrite H35;simpl;unfold bit_rev;rewrite lxor_spec;destruct (bit (k (Typ.interp t_i) v1) i1);destruct (bit (k0 (Typ.interp t_i) v2) i1);[left|right;left|right;right|left];trivial.
 
       admit.
       admit.
 
-      apply wf_t_atom. apply def_t_atom. apply wf_t_atom. apply def_t_atom. apply wf_t_atom. apply def_t_atom. apply wf_t_atom. apply def_t_atom. apply wf_t_atom. apply def_t_atom. apply wf_t_atom. apply def_t_atom. apply wf_t_atom. apply def_t_atom. apply wf_t_atom. apply def_t_atom. apply C.interp_true. apply wf_rho.
 
-
-      intros i2 H0.
-      case_eq (c);intros t; auto using C.interp_true;intro H1.
-      case_eq t;intro H00;auto using C.interp_true.
+      case_eq (c);[intros|intros|intros|intros|intros|intros|intros|intros|intros|intros|intros t H1]; auto using C.interp_true.
+      case_eq t;[intros|intro|intro|intro|intro H2|intro];auto using C.interp_true; subst t.
       case_eq ((length lits == digits + 1) && Lit.is_pos (lits .[ 0]) &&
       forallbi
         (fun i6 l : int =>
@@ -466,7 +484,7 @@ Section Checker.
                           | Auop (UO_index k) h2' =>
                               Lit.is_pos l1 && Lit.is_pos l2 &&
                               negb (Lit.is_pos l) && (j == i6 - 1) &&
-                              (k == j) && (i1 == h1') && (h2' == i2)
+                              (k == j) && (h1 == h1') && (h2' == h2)
                           | _ => false
                           end
                       | _ => false
@@ -478,12 +496,12 @@ Section Checker.
           | _ => false
           end) lits
               );intros H6; auto using C.interp_true.
-      apply andb_true_iff in H6; destruct H6 as (H6,H7);apply andb_true_iff in H6; destruct H6 as (H6,H9); subst t.
+      apply andb_true_iff in H6; destruct H6 as (H6,H7);apply andb_true_iff in H6; destruct H6 as (H6,H9).
 
       rewrite forallbi_spec in H7; unfold C.interp;apply existsb_exists.
       
-      case_eq (interp_atom (t_atom.[i1])); intros t1' v1 H00.
-      case_eq (interp_atom (t_atom.[i2])); intros t2' v2 H01.
+      case_eq (interp_atom (t_atom.[h1])); intros t1' v1 H00.
+      case_eq (interp_atom (t_atom.[h2])); intros t2' v2 H01.
       case_eq (Typ.cast t1' Typ.Tint);intros k1. intro H02.
       case_eq (Typ.cast t2' Typ.Tint);intros k2. intro H03.
       
@@ -493,11 +511,9 @@ Section Checker.
       exists (lits.[0]);split.
       apply to_list_In;rewrite H6;reflexivity.
       
-      unfold Lit.interp. rewrite H9; unfold Var.interp; rewrite rho_interp; rewrite H; simpl;unfold Atom.interp_form_hatom; unfold interp_hatom; rewrite !t_interp_wf.   
-      rewrite H0; simpl; unfold interp_bop; rewrite H1; simpl; rewrite !t_interp_wf.
+      unfold Lit.interp. rewrite H9; unfold Var.interp; rewrite rho_interp; rewrite H; simpl;unfold Atom.interp_form_hatom; unfold interp_hatom; rewrite !t_interp_wf;try (apply wf_t_atom);try (apply def_t_atom).   
+      rewrite H0; simpl; unfold interp_bop; rewrite H1; simpl; rewrite !t_interp_wf;try (apply wf_t_atom);try (apply def_t_atom).
       unfold apply_binop;rewrite H01;rewrite H03; rewrite H00; rewrite H02;simpl; apply Int63Properties.eqb_spec;apply H8.
-      apply wf_t_atom. apply def_t_atom. apply wf_t_atom. apply def_t_atom. apply wf_t_atom. apply def_t_atom.
-
 
       apply Int63Properties.eqb_spec in H6. apply Int63Properties.eqb_false_spec in H8; apply bit_eq_false in H8; inversion H8. destruct H2 as (H10,H11); clear H8.
       exists (lits.[x+1]);split. 
@@ -508,80 +524,132 @@ Section Checker.
       (if x + 1 == 0
        then Lit.is_pos (lits .[ x + 1])
        else
-        match t_form .[ Lit.blit (lits .[ x + 1])] with
-        | Fiff l1 l2 =>
-            match t_form .[ Lit.blit l1] with
-            | Fatom a1 =>
-                match t_form .[ Lit.blit l2] with
-                | Fatom a2 =>
-                    match t_atom .[ a1] with
-                    | Auop (UO_index j) h1' =>
-                        match t_atom .[ a2] with
-                        | Auop (UO_index k) h2' =>
-                            Lit.is_pos l1 && Lit.is_pos l2 &&
-                            negb (Lit.is_pos (lits .[ x + 1])) &&
-                            (j == x + 1 - 1) && (k == j) && (i1 == h1') &&
-                            (h2' == i2)
-                        | _ => false
-                        end
-                    | _ => false
-                    end
-                | _ => false
-                end
-            | _ => false
-            end
-        | _ => false
-        end) = true) -> (if x + 1 == 0
-       then Lit.is_pos (lits .[ x + 1])
-       else
-        match t_form .[ Lit.blit (lits .[ x + 1])] with
-        | Fiff l1 l2 =>
-            match t_form .[ Lit.blit l1] with
-            | Fatom a1 =>
-                match t_form .[ Lit.blit l2] with
-                | Fatom a2 =>
-                    match t_atom .[ a1] with
-                    | Auop (UO_index j) h1' =>
-                        match t_atom .[ a2] with
-                        | Auop (UO_index k) h2' =>
-                            Lit.is_pos l1 && Lit.is_pos l2 &&
-                            negb (Lit.is_pos (lits .[ x + 1])) &&
-                            (j == x + 1 - 1) && (k == j) && (i1 == h1') &&
-                            (h2' == i2)
-                        | _ => false
-                        end
-                    | _ => false
-                    end
-                | _ => false
-                end
-            | _ => false
-            end
-        | _ => false
-        end) = true). intro H13. apply H12; trivial. apply H2 in H12; clear H2.
-        assert (x + 1 == 0 = false) as H7. apply eqb_false_spec; apply not_0_ltb; apply succ_max_int. apply (ltb_trans x digits max_int). apply H11. reflexivity. rewrite H7 in H12.
-        case_eq (t_form .[ Lit.blit (lits .[ x + 1])]); [intros i02 H2|intro H2|intro H2|intros i02 i03 H2|intros i02 H2|intros i02 H2| intros i02 H2| intros i02 i03 H2|intros l1 l2 H2|intros i02 i3 i4 H2]; rewrite H2 in H12; try (apply diff_false_true in H12; inversion H12).
-        case_eq (t_form .[ Lit.blit l1]); [intros a1 H3|intros H3|intro H3|intros a1 a2 H3| intros a1 H3|intros z H3| intros z H3|intros z1 z2 H3|intros z1 z2 H3|intros z1 z2 z3 H3];rewrite H3 in H12; try (apply diff_false_true in H12; inversion H12).
-        case_eq (t_form .[ Lit.blit l2]); [intros a2 H4|intros H4|intro H4|intros z1 z2 H4| intros z2 H4|intros z H4| intros z H4|intros z1 z2 H4|intros z1 z2 H4|intros z1 z2 z3 H4]; rewrite H4 in H12; try (apply diff_false_true in H12; inversion H12).
-        case_eq (t_atom .[a1]); [intros z1 H05|intros u1 h1' H05|intros z3 z1 z2 H05|intros z1 z2 H05|intros z1 z2 H05]; rewrite H05 in H12; try (apply diff_false_true in H12; inversion H12).
-        case_eq (u1); [intro H06|intro H06|intro H06|intro H06|intro H06|intros j H06]; rewrite H06 in H12; try (apply diff_false_true in H12; inversion H12).
-        case_eq (t_atom .[a2]); [intros z1 H07|intros u2 h2' H07|intros z3 z1 z2 H07|intros z1 z2 H07|intros z1 z2 H07]; rewrite H07 in H12; try (apply diff_false_true in H12; inversion H12).
-        case_eq (u2); [intro H08|intro H08|intro H08|intro H08|intro H08|intros k H08]; rewrite H08 in H12; try (apply diff_false_true in H12; inversion H12).
-        apply andb_true_iff in H12; destruct H12 as (H12,H13);apply andb_true_iff in H12; destruct H12 as (H12,H14);apply andb_true_iff in H12; destruct H12 as (H12,H15);apply andb_true_iff in H12; destruct H12 as (H12,H16);apply andb_true_iff in H12; destruct H12 as (H12,H17);apply andb_true_iff in H12; destruct H12 as (H12,H18). 
-        apply negb_true_iff in H17; apply Int63Properties.eqb_spec in H16;apply Int63Properties.eqb_spec in H14;apply Int63Properties.eqb_spec in H15;apply Int63Properties.eqb_spec in H13; subst j;subst k;subst h1'; subst h2'; rewrite <- H06 in H08; subst u2.
-        
-        unfold Lit.interp; rewrite H17; apply negb_true_iff; unfold Var.interp; rewrite rho_interp. rewrite H2; simpl; unfold Lit.interp. rewrite H12;rewrite H18; unfold Var.interp; rewrite !rho_interp. rewrite H3; rewrite H4; simpl; unfold Atom.interp_form_hatom; unfold interp_hatom; rewrite !t_interp_wf.
-        rewrite H07; rewrite H05; simpl; unfold interp_uop. rewrite H06; rewrite !t_interp_wf. 
-        assert (x = x+1-1) as H5. rewrite <- to_Z_eq; rewrite (to_Z_sub_1 (x+1) 0). rewrite (to_Z_add_1 x max_int); intuition. apply (ltb_trans x digits max_int). apply H11. reflexivity. apply eqb_false_spec in H7; apply not_0_ltb in H7; apply H7. rewrite <- H5; unfold bit_rev; apply Bool.eqb_false_iff.
-        unfold apply_unop;rewrite H00;rewrite H01;rewrite H02;rewrite H03;simpl;apply H10.
-        apply wf_t_atom. apply def_t_atom. apply wf_t_atom. apply def_t_atom. apply wf_t_atom. apply def_t_atom. apply wf_t_atom. apply def_t_atom.
-        reflexivity. apply H11.
-        
+         match t_form .[ Lit.blit (lits .[ x + 1])] with
+         | Fiff l1 l2 =>
+           match t_form .[ Lit.blit l1] with
+           | Fatom a1 =>
+             match t_form .[ Lit.blit l2] with
+             | Fatom a2 =>
+               match t_atom .[ a1] with
+               | Auop (UO_index j) h1' =>
+                 match t_atom .[ a2] with
+                 | Auop (UO_index k) h2' =>
+                   Lit.is_pos l1 && Lit.is_pos l2 &&
+                   negb (Lit.is_pos (lits .[ x + 1])) &&
+                   (j == x + 1 - 1) && (k == j) && (h1 == h1') &&
+                   (h2' == h2)
+                 | _ => false
+                 end
+               | _ => false
+               end
+             | _ => false
+             end
+           | _ => false
+           end
+         | _ => false
+         end) = true) -> (
+         if x + 1 == 0
+         then Lit.is_pos (lits .[ x + 1])
+         else
+           match t_form .[ Lit.blit (lits .[ x + 1])] with
+           | Fiff l1 l2 =>
+             match t_form .[ Lit.blit l1] with
+             | Fatom a1 =>
+               match t_form .[ Lit.blit l2] with
+               | Fatom a2 =>
+                 match t_atom .[ a1] with
+                 | Auop (UO_index j) h1' =>
+                   match t_atom .[ a2] with
+                   | Auop (UO_index k) h2' =>
+                     Lit.is_pos l1 && Lit.is_pos l2 &&
+                     negb (Lit.is_pos (lits .[ x + 1])) &&
+                     (j == x + 1 - 1) && (k == j) && (h1 == h1') &&
+                     (h2' == h2)
+                   | _ => false
+                   end
+                 | _ => false
+                 end
+               | _ => false
+               end
+             | _ => false
+             end
+           | _ => false
+           end) = true). 
+      intro H13. apply H12; trivial. apply H2 in H12; clear H2.
+      assert (x + 1 == 0 = false) as H7. apply eqb_false_spec; apply not_0_ltb; apply succ_max_int. apply (ltb_trans x digits max_int). apply H11. reflexivity. rewrite H7 in H12.
+      case_eq (t_form .[ Lit.blit (lits .[ x + 1])]); [intros i02 H2|intro H2|intro H2|intros i02 i03 H2|intros i02 H2|intros i02 H2| intros i02 H2| intros i02 i03 H2|intros l1 l2 H2|intros i02 i3 i4 H2]; rewrite H2 in H12; try (apply diff_false_true in H12; inversion H12).
+      case_eq (t_form .[ Lit.blit l1]); [intros a1 H3|intros H3|intro H3|intros a1 a2 H3| intros a1 H3|intros z H3| intros z H3|intros z1 z2 H3|intros z1 z2 H3|intros z1 z2 z3 H3];rewrite H3 in H12; try (apply diff_false_true in H12; inversion H12).
+      case_eq (t_form .[ Lit.blit l2]); [intros a2 H4|intros H4|intro H4|intros z1 z2 H4| intros z2 H4|intros z H4| intros z H4|intros z1 z2 H4|intros z1 z2 H4|intros z1 z2 z3 H4]; rewrite H4 in H12; try (apply diff_false_true in H12; inversion H12).
+      case_eq (t_atom .[a1]); [intros z1 H05|intros u1 h1' H05|intros z3 z1 z2 H05|intros z1 z2 H05|intros z1 z2 H05]; rewrite H05 in H12; try (apply diff_false_true in H12; inversion H12).
+      case_eq (u1); [intro H06|intro H06|intro H06|intro H06|intro H06|intros j H06]; rewrite H06 in H12; try (apply diff_false_true in H12; inversion H12).
+      case_eq (t_atom .[a2]); [intros z1 H07|intros u2 h2' H07|intros z3 z1 z2 H07|intros z1 z2 H07|intros z1 z2 H07]; rewrite H07 in H12; try (apply diff_false_true in H12; inversion H12).
+      case_eq (u2); [intro H08|intro H08|intro H08|intro H08|intro H08|intros k H08]; rewrite H08 in H12; try (apply diff_false_true in H12; inversion H12).
+      apply andb_true_iff in H12; destruct H12 as (H12,H13);apply andb_true_iff in H12; destruct H12 as (H12,H14);apply andb_true_iff in H12; destruct H12 as (H12,H15);apply andb_true_iff in H12; destruct H12 as (H12,H16);apply andb_true_iff in H12; destruct H12 as (H12,H17);apply andb_true_iff in H12; destruct H12 as (H12,H18). 
+      apply negb_true_iff in H17; apply Int63Properties.eqb_spec in H16;apply Int63Properties.eqb_spec in H14;apply Int63Properties.eqb_spec in H15;apply Int63Properties.eqb_spec in H13; subst j;subst k;subst h1'; subst h2'; rewrite <- H06 in H08; subst u2.
+      
+      unfold Lit.interp; rewrite H17; apply negb_true_iff; unfold Var.interp; rewrite rho_interp. rewrite H2; simpl; unfold Lit.interp. rewrite H12;rewrite H18; unfold Var.interp; rewrite !rho_interp. rewrite H3; rewrite H4; simpl; unfold Atom.interp_form_hatom; unfold interp_hatom; rewrite !t_interp_wf;try (apply wf_t_atom);try (apply def_t_atom).
+      rewrite H07; rewrite H05; simpl; unfold interp_uop. rewrite H06; rewrite !t_interp_wf;try (apply wf_t_atom);try (apply def_t_atom). 
+      assert (x = x+1-1) as H5. rewrite <- to_Z_eq; rewrite (to_Z_sub_1 (x+1) 0). rewrite (to_Z_add_1 x max_int); intuition. apply (ltb_trans x digits max_int). apply H11. reflexivity. apply eqb_false_spec in H7; apply not_0_ltb in H7; apply H7. rewrite <- H5; unfold bit_rev; apply Bool.eqb_false_iff.
+      unfold apply_unop;rewrite H00;rewrite H01;rewrite H02;rewrite H03;simpl;apply H10.
+      reflexivity. apply H11.
+      
+      
+      (* Ces deux admit correspondent aux case_eq (Typ.cast t1' Typ.Tint) et case_eq (Typ.cast t2' Typ.Tint)*)
+      admit.
+      admit.
+    Qed.
+    
+    Lemma valid_check_BuildDefInt2 : forall lits, C.valid rho (check_BuildDefInt2 lits).
+    Proof.
+      unfold check_BuildDefInt2,C.valid; intros lits.
+      
+      case_eq (t_form .[ Lit.blit (lits .[ 0])]); [intros a H|intro H|intro H|intros z1 z2 H|intros z1 H|intros z1 H|intros z1 H|intros z1 z2 H|intros z1 z2 H|intros z1 z2 z3 H]; auto using C.interp_true.
+      case_eq (t_atom.[a]);[intros z1 H0|intros c hxor H0|intros z1 z2 z3 H0|intros z1 z2 H0|intros z1 z2 H0]; auto using C.interp_true.
+      case_eq c;intro i1;auto using C.interp_true;intro H1.
+      case_eq (t_atom.[hxor]);[intros z1 H2|intros z1 z2 H2|intros b h1 h2 H2|intros z1 z2 H2|intros z1 z2 H2];auto using C.interp_true.
+      case_eq b; intro H3;auto using C.interp_true.
+      case_eq (length lits == 3); intros H4; auto using C.interp_true. 
+      case_eq (t_form .[ Lit.blit (lits .[ 1])]);[intros a1 H5|intros|intros|intros|intros|intros|intros|intros|intros|intros]; auto using C.interp_true.
+      case_eq (t_form .[ Lit.blit (lits .[ 2])]);[intros a2 H6|intros|intros|intros|intros|intros|intros|intros|intros|intros]; auto using C.interp_true.
+      case_eq (t_atom .[ a1]);[intros|intros c1 h1' H7|intros|intros|intros]; auto using C.interp_true.
+      case_eq c1;intro i2;auto using C.interp_true; intro H8.
+      case_eq (t_atom .[ a2]);[intros|intros c2 h2' H9|intros|intros|intros]; auto using C.interp_true.
+      case_eq c2;intro i3;auto using C.interp_true;intro H10.
+      case_eq ((h1' == h1) && (h2 == h2') && (i1 == i2) && (i2 == i3) && Lit.is_pos (lits .[ 1]) && Lit.is_pos (lits .[ 2])); auto using C.interp_true;intros H23.
+      apply andb_true_iff in H23; destruct H23 as (H23,H31);apply andb_true_iff in H23; destruct H23 as (H23,H26);apply andb_true_iff in H23; destruct H23 as (H23,H27);apply andb_true_iff in H23; destruct H23 as (H23,H29);apply andb_true_iff in H23; destruct H23 as (H23,H30).
+      apply Int63Properties.eqb_spec in H23;apply Int63Properties.eqb_spec in H27;apply Int63Properties.eqb_spec in H29;apply Int63Properties.eqb_spec in H30; subst h1';subst h2';subst i2;subst i3. rewrite <- H1 in H10;rewrite <- H1 in H8; subst c1; subst c2.
+      
+      case_eq (Lit.is_pos (lits.[0]));intro H14.
+      
+      simpl; rewrite orb_false_r; apply orb_true_iff; rewrite orb_true_iff.
+      unfold Lit.interp; rewrite H31; rewrite H14; rewrite Lit.is_pos_neg; rewrite H26; simpl; unfold Var.interp; rewrite !rho_interp; rewrite Lit.blit_neg; rewrite H;rewrite H5;rewrite H6; simpl; unfold Atom.interp_form_hatom; unfold interp_hatom; rewrite !t_interp_wf;try (apply wf_t_atom);try (apply def_t_atom).
+      rewrite H0;rewrite H7;rewrite H9; simpl; unfold interp_uop; rewrite H1; rewrite !t_interp_wf;try (apply wf_t_atom);try (apply def_t_atom).
+      rewrite H2; simpl; rewrite !t_interp_wf;try (apply wf_t_atom);try (apply def_t_atom).
+      unfold interp_bop; rewrite H3;simpl; unfold apply_binop.
+      case_eq (interp_atom (t_atom.[h1])); intros t1' v1 H32.
+      case_eq (interp_atom (t_atom.[h2])); intros t2' v2 H33.
+      case_eq (Typ.cast t1' Typ.Tint); intros k. intro H34.
+      case_eq (Typ.cast t2' Typ.Tint); intros k0. intro H35.
+      simpl;rewrite H34;rewrite H35;simpl;unfold bit_rev;rewrite lxor_spec;destruct (bit (k (Typ.interp t_i) v1) i1);destruct (bit (k0 (Typ.interp t_i) v2) i1);[right;right|left|left|right;left];trivial.
 
-(* Ces deux admit correspondent aux case_eq (Typ.cast t1' Typ.Tint) et case_eq (Typ.cast t2' Typ.Tint)*)
-        admit.
-        admit.
-   Qed.
- 
+      admit.
+      admit.
+      
+      simpl; rewrite orb_false_r; apply orb_true_iff; rewrite orb_true_iff.
+      unfold Lit.interp; rewrite !Lit.is_pos_neg;rewrite H26; rewrite H14;rewrite H31; simpl; unfold Var.interp; rewrite !rho_interp;rewrite !Lit.blit_neg;rewrite H;rewrite H5;rewrite H6; simpl; unfold Atom.interp_form_hatom; unfold interp_hatom; rewrite !t_interp_wf;try (apply wf_t_atom);try (apply def_t_atom).
+      rewrite H0;rewrite H7;rewrite H9; simpl; unfold interp_uop; rewrite H1; rewrite !t_interp_wf;try (apply wf_t_atom);try (apply def_t_atom).
+      rewrite H2; simpl; rewrite !t_interp_wf;try (apply wf_t_atom);try (apply def_t_atom).
+      unfold interp_bop; rewrite H3;simpl; unfold apply_binop.
+      case_eq (interp_atom (t_atom.[h1])); intros t1' v1 H32.
+      case_eq (interp_atom (t_atom.[h2])); intros t2' v2 H33.
+      case_eq (Typ.cast t1' Typ.Tint); intros k. intro H34.
+      case_eq (Typ.cast t2' Typ.Tint); intros k0. intro H35.
+      simpl;rewrite H34;rewrite H35;simpl;unfold bit_rev;rewrite lxor_spec;destruct (bit (k (Typ.interp t_i) v1) i1);destruct (bit (k0 (Typ.interp t_i) v2) i1);[left|right;right|right;left|left];trivial.
+
+      admit.
+      admit.
+    Qed.
+    
   End Proof.
   
 End Checker.
